progress on ed25519

code/experimental/ed25519/Hacl.Impl.Ed25519.RecoverX.fst
@@ -2,96 +2,190 @@ module Hacl.Impl.Ed25519.RecoverX
 
 open FStar.Buffer
 open FStar.UInt64
-open Hacl.Spec.BignumQ.Eval
+open Hacl.Bignum25519
+
+#reset-options "--max_fuel 0 --z3rlimit 20"
+
 
 let elemB = b:buffer Hacl.UInt64.t{length b = 5}
 
+open FStar.Mul
+
+let norm h (x:elemB{live h x}) : GTot Type0 =
+  live h x /\ red_51 (as_seq h x) /\ (let s = as_seq h x in
+  v (Seq.index s 0) + pow2 51 * v (Seq.index s 1) + pow2 102 * v (Seq.index s 2) + pow2 153 * v (Seq.index s 3) + pow2 204 * v (Seq.index s 4) < Spec.Curve25519.prime)
+
+
+private
+val make_zero:
+  b:elemB ->
+  Stack unit
+    (requires (fun h -> live h b))
+    (ensures (fun h0 _ h1 -> live h1 b /\ modifies_1 b h0 h1 /\ seval (as_seq h1 b) == 0
+      /\ norm h1 b
+      /\ Hacl.Bignum25519.red_513 (as_seq h1 b)))
+let make_zero b =
+  let zero = Hacl.Cast.uint64_to_sint64 0uL in
+  Hacl.Lib.Create64.make_h64_5 b zero zero zero zero zero;
+  let h = ST.get() in
+  lemma_reveal_seval (as_seq h b);
+  assert_norm(pow2 51 = 0x8000000000000);
+  lemma_intro_red_51 (as_seq h b);
+  lemma_red_51_is_red_513 (as_seq h b)
+
+
+private
+val make_one:
+  b:elemB ->
+  Stack unit
+    (requires (fun h -> live h b))
+    (ensures (fun h0 _ h1 -> live h1 b /\ modifies_1 b h0 h1 /\ seval (as_seq h1 b) == 1
+      /\ Hacl.Bignum25519.red_513 (as_seq h1 b)))
+let make_one b =
+  let zero = Hacl.Cast.uint64_to_sint64 0uL in
+  let one  = Hacl.Cast.uint64_to_sint64 1uL in
+  Hacl.Lib.Create64.make_h64_5 b one zero zero zero zero;
+  let h = ST.get() in
+  lemma_reveal_seval (as_seq h b);
+  assert_norm(pow2 51 = 0x8000000000000);
+  lemma_intro_red_51 (as_seq h b);
+  lemma_red_51_is_red_513 (as_seq h b)
+
+
+#reset-options "--max_fuel 0 --z3rlimit 20"
+
+[@ "substitute"]
 private
 val recover_x_step_1:
   x2:elemB ->
-  y:elemB ->
+  y:elemB{disjoint x2 y} ->
   Stack unit
-    (requires (fun h -> live h x2 /\ live h y))
-    (ensures (fun h0 _ h1 -> live h1 x2 /\ live h0 y /\ modifies_1 x2 h0 h1))
+    (requires (fun h -> live h x2 /\ live h y /\ red_51 (as_seq h y)))
+    (ensures (fun h0 _ h1 -> live h1 x2 /\ live h0 y /\ modifies_1 x2 h0 h1 /\
+      (let s = as_seq h1 x2 in
+       red_51 s /\
+       FStar.Mul.(Hacl.UInt64.(v (Seq.index s 0)
+                               + pow2 51 * v (Seq.index s 1)
+                               + pow2 102 * v (Seq.index s 2)
+                               + pow2 153 * v (Seq.index s 3)
+                               + pow2 204 * v (Seq.index s 4) < Spec.Curve25519.prime))) /\
+      (let y = seval (as_seq h0 y) in
+       let x2 = seval (as_seq h1 x2) in
+       Spec.Ed25519.(Spec.Curve25519.(
+         x2 == ((y `fmul` y) `fsub` 1) `fmul` (modp_inv ((d `fmul` (y `fmul` y)) `fadd` one)))))))
+#reset-options "--max_fuel 0 --z3rlimit 200"
+[@ "substitute"]
 let recover_x_step_1 x2 y =
   push_frame();
-  let zero = (Hacl.Cast.uint64_to_sint64 0uL) in
-  let one' = (Hacl.Cast.uint64_to_sint64 1uL) in
   let tmp = create (Hacl.Cast.uint64_to_sint64 0uL) 25ul in
   let one = Buffer.sub tmp 0ul 5ul in
   let y2  = Buffer.sub tmp 5ul 5ul in
   let dyyi = Buffer.sub tmp 10ul 5ul in
   let dyy = Buffer.sub tmp 15ul 5ul in
-  Hacl.Lib.Create64.make_h64_5 one one' zero zero zero zero;
-  Hacl.Bignum25519.fsquare y2 y;
-  Hacl.Bignum25519.times_d dyy y2;
-  Hacl.Bignum25519.fsum dyy one;
-  Hacl.Bignum25519.inverse dyyi dyy;
-  Hacl.Bignum25519.fdifference one y2;
-  Hacl.Bignum25519.fmul x2 one dyyi;
-  Hacl.Bignum25519.reduce x2;  
+  let h0 = ST.get() in
+  make_one one;
+  let h1 = ST.get() in
+  lemma_red_51_is_red_5413 (as_seq h1 y);
+  Hacl.Bignum25519.fsquare y2 y; // y2 = y `fmul` y
+  Hacl.Bignum25519.times_d dyy y2; // dyy = d `fmul` (y `fmul` y)
+  Hacl.Bignum25519.fsum dyy one;   // dyy = (d `fmul` (y `fmul` y)) `fadd` one
+  let h4 = ST.get() in
+  lemma_red_53_is_red_5413 (as_seq h4 dyy);
+  Hacl.Bignum25519.reduce_513 dyy;
+  Hacl.Bignum25519.inverse dyyi dyy; // dyyi = modp_inv ((d `fmul` (y `fmul` y)) `fadd` one)
+  Hacl.Bignum25519.fdifference one y2; // one = (y `fmul` y) `fsub` 1
+  let h7 = ST.get() in
+  lemma_red_513_is_red_53 (as_seq h7 dyyi);
+  Hacl.Bignum25519.fmul x2 dyyi one; //
+  Hacl.Bignum25519.reduce x2;
   pop_frame()
 
 
-(* val compare: *)
-(*   x:elemB -> *)
-(*   y:elemB -> *)
-(*   Stack bool *)
-(*     (requires (fun h -> live h x /\ live h y)) *)
-(*     (ensures (fun h0 b h1 -> h0 == h1 /\ live h0 x /\ live h0 y /\ *)
-(*       b <==> (as_seq h0 x == as_seq h0 y))) *)
-(* let compare x y = *)
-(*   let x0 = x.(0ul) in *)
-(*   let x1 = x.(1ul) in *)
-(*   let x2 = x.(2ul) in *)
-(*   let x3 = x.(3ul) in *)
-(*   let x4 = x.(4ul) in *)
-(*   let y0 = y.(0ul) in *)
-(*   let y1 = y.(1ul) in *)
-(*   let y2 = y.(2ul) in *)
-(*   let y3 = y.(3ul) in *)
-(*   let y4 = y.(4ul) in *)
-(*   FStar.UInt64.(x0 =^ y0 && x1 =^ y1 && x2 =^ y2 && x3 =^ y3 && x4 =^ y4) *)
+#reset-options "--max_fuel 0 --z3rlimit 20"
 
 private
 val is_0:
   x:elemB ->
   Stack bool
-    (requires (fun h -> live h x /\ Hacl.Bignum25519.red_51 (as_seq h x)))
+    (requires (fun h -> live h x /\ Hacl.Bignum25519.red_51 (as_seq h x) /\
+      (let s = as_seq h x in
+       FStar.Mul.(v (Seq.index s 0) + pow2 51 * v (Seq.index s 1)
+                  + pow2 102 * v (Seq.index s 2) + pow2 153 * v (Seq.index s 3)
+                  + pow2 204 * v (Seq.index s 4) < Spec.Curve25519.prime)) ))
     (ensures (fun h0 b h1 -> h0 == h1 /\ live h0 x /\
-      b <==> (Hacl.Spec.Bignum.Bigint.seval (as_seq h0 x) == 0)))
+      (b <==> (seval (as_seq h0 x) = 0))))
+#reset-options "--max_fuel 0 --z3rlimit 200"
 let is_0 x =
   let x0 = x.(0ul) in
   let x1 = x.(1ul) in
   let x2 = x.(2ul) in
   let x3 = x.(3ul) in
   let x4 = x.(4ul) in
+  let h = ST.get() in
+  lemma_reveal_seval (as_seq h x);
+  Math.Lemmas.modulo_lemma (let s = as_seq h x in
+       FStar.Mul.(v (Seq.index s 0) + pow2 51 * v (Seq.index s 1)
+                  + pow2 102 * v (Seq.index s 2) + pow2 153 * v (Seq.index s 3)
+                  + pow2 204 * v (Seq.index s 4))) Spec.Curve25519.prime;
   FStar.UInt64.(x0 =^ 0uL && x1 =^ 0uL && x2 =^ 0uL && x3 =^ 0uL && x4 =^ 0uL)
+
+
+#reset-options "--max_fuel 0 --z3rlimit 20"
 
 private
 val mul_modp_sqrt_m1:
   x:elemB ->
   Stack unit
-    (requires (fun h -> live h x /\ Hacl.Bignum25519.red_51 (as_seq h x) ))
+    (requires (fun h -> live h x /\ red_513 (as_seq h x) ))
     (ensures (fun h0 _ h1 -> live h1 x /\ live h0 x /\ modifies_1 x h0 h1
-      /\ Hacl.Bignum25519.red_51 (as_seq h0 x) /\ Hacl.Bignum25519.red_51 (as_seq h1 x) /\
-      Hacl.Spec.Bignum.Bigint.seval (as_seq h1 x)
-      == Spec.Curve25519.(Hacl.Spec.Bignum.Bigint.seval (as_seq h0 x) `fmul` (Spec.Ed25519.modp_sqrt_m1))
+      /\ red_513 (as_seq h0 x) /\ red_513 (as_seq h1 x) /\
+      seval (as_seq h1 x)
+      == Spec.Curve25519.(seval (as_seq h0 x) `fmul` (Spec.Ed25519.modp_sqrt_m1))
+      (* (let s = as_seq h1 x in *)
+      (*  FStar.Mul.(Hacl.UInt64.(v (Seq.index s 0) *)
+      (*                          + pow2 51 * v (Seq.index s 1) *)
+      (*                          + pow2 102 * v (Seq.index s 2) *)
+      (*                          + pow2 153 * v (Seq.index s 3) *)
+      (*                          + pow2 204 * v (Seq.index s 4) < Spec.Curve25519.prime))) *)
     ))
+#reset-options "--max_fuel 0 --z3rlimit 200"
 let mul_modp_sqrt_m1 x =
+  let open FStar.Mul in
+  assert_norm(pow2 51 = 0x8000000000000);
+  assert_norm((0x00061b274a0ea0b0 + pow2 51 * 0x0000d5a5fc8f189d + pow2 102 *  0x0007ef5e9cbd0c60 + pow2 153 *  0x00078595a6804c9e + pow2 204 * 0x0002b8324804fc1d) % (pow2 255 - 19) = Spec.Ed25519.modp_sqrt_m1);
   push_frame();
   let sqrt_m1 = create 0uL 5ul in
   Hacl.Lib.Create64.make_h64_5 sqrt_m1 0x00061b274a0ea0b0uL 0x0000d5a5fc8f189duL 0x0007ef5e9cbd0c60uL 0x00078595a6804c9euL 0x0002b8324804fc1duL;
+  let h = ST.get() in
+  lemma_intro_red_51 (as_seq h sqrt_m1);
+  lemma_reveal_seval (as_seq h sqrt_m1);
+  assert(seval (as_seq h sqrt_m1) = Spec.Ed25519.modp_sqrt_m1);
+  lemma_red_513_is_red_53 (as_seq h x);
+  lemma_red_51_is_red_5413 (as_seq h sqrt_m1);
   Hacl.Bignum25519.fmul x x sqrt_m1;
-  Hacl.Bignum25519.reduce x;
+  (* Hacl.Bignum25519.reduce x; *)
   pop_frame()
+
+
+#reset-options "--max_fuel 0 --z3rlimit 20"
 
 val gte_q:
   x:elemB ->
   Stack bool
-    (requires (fun h -> live h x))
-    (ensures (fun h0 _ h1 -> live h0 x /\ h0 == h1))
+    (requires (fun h -> live h x /\ red_51 (as_seq h x)))
+    (ensures (fun h0 b h1 -> live h0 x /\ h0 == h1
+     /\ (b <==> (let s = as_seq h0 x in
+       FStar.Mul.(v (Seq.index s 0) + pow2 51 * v (Seq.index s 1)
+                  + pow2 102 * v (Seq.index s 2) + pow2 153 * v (Seq.index s 3)
+                  + pow2 204 * v (Seq.index s 4)) >= pow2 255 - 19)) ))
 let gte_q x =
+  let h = ST.get() in
+  lemma_reveal_red_51 (as_seq h x);
+  assert_norm(pow2 51 = 0x8000000000000);
+  assert_norm(pow2 102 = 0x40000000000000000000000000);
+  assert_norm(pow2 153 = 0x200000000000000000000000000000000000000);
+  assert_norm(pow2 204 = 0x1000000000000000000000000000000000000000000000000000);
+  assert_norm(pow2 255 - 19 = 0x7fffffffffffffffffffffffffffffffffffffffffffffffffffffffffffffed);
   let x0 = x.(0ul) in
   let x1 = x.(1ul) in
   let x2 = x.(2ul) in
@@ -99,14 +193,169 @@ let gte_q x =
   let x4 = x.(4ul) in
   FStar.UInt64.(x0 >=^ 0x7ffffffffffeduL && x1 =^ 0x7ffffffffffffuL && x2 =^ 0x7ffffffffffffuL && x3 =^ 0x7ffffffffffffuL && x4 =^ 0x7ffffffffffffuL)
 
-val recover_x:
+
+open FStar.Mul
+
+[@ "substitute"]
+private
+val copy:
+  src:elemB ->
+  dest:elemB{disjoint src dest} ->
+  Stack unit
+    (requires (fun h -> live h src /\ live h dest))
+    (ensures (fun h0 _ h1 -> live h0 src /\ live h1 dest /\ modifies_1 dest h0 h1 /\
+      as_seq h1 dest == as_seq h0 src))
+[@ "substitute"]
+let copy src dest =
+  let h0 = ST.get() in
+  blit src 0ul dest 0ul 5ul;
+  let h1 = ST.get() in
+  Seq.lemma_eq_intro (Seq.slice (as_seq h0 src) 0 5) (as_seq h0 src);
+  Seq.lemma_eq_intro (Seq.slice (as_seq h1 dest) 0 5) (as_seq h1 dest)
+
+
+private
+let lemma_mul_5 (a:nat) (b:nat) (c:nat) (d:nat) (e:nat) : Lemma
+  (a + pow2 51 * b + pow2 102 * c + pow2 153 * e + pow2 204 * e >= 0)
+  = ()
+
+
+[@ "substitute"]
+private
+val fdifference_norm:
   x:elemB ->
   y:elemB{disjoint x y} ->
-  sign:Hacl.UInt64.t ->
+  Stack unit
+    (requires (fun h -> live h x /\ live h y /\ red_513 (as_seq h y) /\ red_513 (as_seq h x)))
+    (ensures (fun h0 _ h1 -> live h0 x /\ live h0 y /\ live h1 x /\ live h1 y /\ red_513 (as_seq h0 x)
+      /\ red_513 (as_seq h0 y)
+      /\ modifies_1 x h0 h1 /\ red_51 (as_seq h1 x) /\
+      (let s = as_seq h1 x in
+       FStar.Mul.(Hacl.UInt64.(v (Seq.index s 0)
+                               + pow2 51 * v (Seq.index s 1)
+                               + pow2 102 * v (Seq.index s 2)
+                               + pow2 153 * v (Seq.index s 3)
+                               + pow2 204 * v (Seq.index s 4) < Spec.Curve25519.prime))) /\
+      seval (as_seq h1 x) = Spec.Curve25519.(seval (as_seq h0 y) `fsub` seval (as_seq h0 x))
+    ))
+[@ "substitute"]
+let fdifference_norm x y =
+  fdifference x y;
+  reduce_513 x;
+  reduce x
+
+
+private let lemma_distr_4 a b c d e : Lemma (a * (b + c + d + e) == a * b + a * c + a * d + a * e)
+  = Math.Lemmas.distributivity_add_right a (b + c + d) e;
+    Math.Lemmas.distributivity_add_right a (b + c) d;
+    Math.Lemmas.distributivity_add_right a (b) c
+
+
+private let lemma_x_mod_2 (a:nat) (b:nat) (c:nat) (d:nat) (e:nat) :
+  Lemma ((a + pow2 51 * b + pow2 102 * c + pow2 153 * d + pow2 204 * e) % 2 = a % 2)
+  = assert_norm(pow2 51 = 2 * pow2 50);
+    assert_norm(pow2 102 = 2 * pow2 101);
+    assert_norm(pow2 153 = 2 * pow2 152);
+    assert_norm(pow2 204 = 2 * pow2 203);
+    lemma_distr_4 2 (pow2 50 * b) (pow2 101 * c) (pow2 152 * d) (pow2 203 * e);
+    Math.Lemmas.paren_mul_right 2 (pow2 50) b;
+    Math.Lemmas.paren_mul_right 2 (pow2 101) c;
+    Math.Lemmas.paren_mul_right 2 (pow2 152) d;
+    Math.Lemmas.paren_mul_right 2 (pow2 203) e;
+    Math.Lemmas.modulo_addition_lemma a 2 ((pow2 50 * b)+(pow2 101 * c)+(pow2 152 * d)+(pow2 203 * e))
+
+[@ "substitute"]
+private val x_mod_2:
+  x:felem ->
+  Stack Hacl.UInt64.t
+    (requires (fun h -> live h x /\ red_51 (as_seq h x) /\
+      (let s = as_seq h x in
+       FStar.Mul.(Hacl.UInt64.(v (Seq.index s 0)
+                               + pow2 51 * v (Seq.index s 1)
+                               + pow2 102 * v (Seq.index s 2)
+                               + pow2 153 * v (Seq.index s 3)
+                               + pow2 204 * v (Seq.index s 4) < pow2 255 - 19)))))
+    (ensures (fun h0 z h1 -> h0 == h1 /\ live h0 x /\ v z = seval (as_seq h0 x) % 2))
+[@ "substitute"]
+let x_mod_2 x =
+  let h = ST.get() in
+  Hacl.Bignum25519.lemma_reveal_seval (as_seq h x);
+  Math.Lemmas.modulo_lemma (let s = as_seq h x in v (Seq.index s 0)
+                               + pow2 51 * v (Seq.index s 1)
+                               + pow2 102 * v (Seq.index s 2)
+                               + pow2 153 * v (Seq.index s 3)
+                               + pow2 204 * v (Seq.index s 4)) Spec.Curve25519.prime;
+  lemma_x_mod_2 (v (get h x 0)) (v (get h x 1)) (v (get h x 2)) (v (get h x 3)) (v (get h x 4));
+  let x0 = x.(0ul) in
+  let z  = x0 &^ 1uL in
+  assert_norm(pow2 1 = 2);
+  UInt.logand_mask (v x0) 1;
+  z
+
+
+let lemma_modifies_2 #a #a' h (b:buffer a{live h b}) (b':buffer a'{live h b'}) :
+  Lemma (modifies_2 b b' h h)
+  = lemma_intro_modifies_2 b b' h h
+
+let lemma_modifies_1 #a h (b:buffer a{live h b}) :
+  Lemma (modifies_1 b h h)
+  = lemma_intro_modifies_1 b h h
+
+
+val recover_x_step_2:
+  x:elemB ->
+  sign:Hacl.UInt64.t{v sign < 2} ->
+  x2:elemB{disjoint x x2} ->
   Stack bool
-    (requires (fun h -> live h x /\ live h y))
-    (ensures (fun h0 _ h1 -> live h1 x /\ live h0 y /\ modifies_1 x h0 h1))
-let recover_x x y sign =
+    (requires (fun h -> live h x2 /\ live h x /\
+      (let s = as_seq h x2 in
+       red_51 s /\
+       FStar.Mul.(Hacl.UInt64.(v (Seq.index s 0)
+                               + pow2 51 * v (Seq.index s 1)
+                               + pow2 102 * v (Seq.index s 2)
+                               + pow2 153 * v (Seq.index s 3)
+                               + pow2 204 * v (Seq.index s 4) < Spec.Curve25519.prime))) ))
+    (ensures (fun h0 z h1 -> live h0 x2 /\ live h0 x /\ live h1 x /\ live h1 x2 /\
+      (let x2 = as_seq h0 x2 in
+       if seval x2 = 0 && v sign = 0
+       then (modifies_1 x h0 h1 /\ norm h1 x /\ seval (as_seq h1 x) = 0 /\ z == true)
+       else if seval x2 = 0 && v sign = 1
+       then (h0 == h1 /\ z == false)
+       else (h0 == h1 /\ z == true))))
+let recover_x_step_2 x sign x2 =
+  let x2_is_0 = is_0 x2 in
+  if x2_is_0 then (
+    if sign =^ 0uL then (
+      make_zero x;
+      true
+    ) else false
+  ) else true
+
+
+
+#reset-options "--max_fuel 0 --z3rlimit 100"
+
+val recover_x_:
+  x:elemB ->
+  y:elemB{disjoint x y} ->
+  sign:UInt64.t{v sign = 0 \/ v sign = 1} ->
+  tmp:buffer Hacl.UInt64.t{length tmp = 20} ->
+  Stack bool
+    (requires (fun h -> live h x /\ live h y /\ red_51 (as_seq h y)))
+    (ensures (fun h0 z h1 -> live h1 x /\ live h0 y /\ modifies_1 x h0 h1 /\
+      (let op_String_Access = Seq.index in
+       let y = as_seq h0 y in
+       let y:nat = v y.[0] + pow2 51 * v y.[1] + pow2 102 * v y.[2] + pow2 153 * v y.[3]
+               + pow2 204 * v y.[4] in
+       let x = as_seq h1 x in
+       let sign = (v sign = 1) in
+       let res  = Spec.Ed25519.recover_x y sign in True)
+       (* (z <==> Some? res) *)
+       (* /\ (Some? res ==> (seval x = Some?.v res /\ red_51 x))) *)
+      ))
+#reset-options "--max_fuel 0 --z3rlimit 500"
+let recover_x_ x y sign =
+  assert_norm(pow2 32 = 0x100000000);
   push_frame();
   let tmp = create 0uL 20ul in
   let x2  = Buffer.sub tmp 0ul 5ul in
@@ -115,35 +364,119 @@ let recover_x x y sign =
   let t1  = Buffer.sub tmp 15ul 5ul in
   let b = gte_q y in
   let res =
-  if b then false
-  else (
+  if b then (
+    let hf = ST.get() in
+    lemma_modifies_2 hf x tmp;
+    false
+  ) else (
+    let h = ST.get() in
+    lemma_reveal_seval (as_seq h y);
     recover_x_step_1 x2 y;
     Hacl.Impl.Ed25519.Pow2_252m2.pow2_252m2 x3 x2;
+    let h' = ST.get() in
+    lemma_red_513_is_red_5413 (as_seq h' x3);
     Hacl.Bignum25519.fsquare t0 x3;
-    blit x2 0ul t1 0ul 5ul;
-    Hacl.Bignum25519.fdifference t1 t0;
-    Hacl.Bignum25519.reduce t1;
+    copy x2 t1;
+    fdifference_norm t1 t0;
     let t1_is_0 = is_0 t1 in
     if t1_is_0 then ()
     else (
       mul_modp_sqrt_m1 x3
     );
     Hacl.Bignum25519.fsquare t0 x3;
-    blit x2 0ul t1 0ul 5ul;
-    Hacl.Bignum25519.fdifference t1 t0;
-    Hacl.Bignum25519.reduce t1;
+    copy x2 t1;
+    fdifference_norm t1 t0;
+    Hacl.Bignum25519.reduce x3;
     let t1_is_0 = is_0 t1 in
     if t1_is_0 then (
-      let x0 = x3.(0ul) &^ 1uL in
+      let x0 = x_mod_2 x3 in
+      (* let x0 = x3.(0ul) &^ 1uL in *)
       if not(x0 =^ sign) then (
-        Hacl.Lib.Create64.make_h64_5 t0 0uL 0uL 0uL 0uL 0uL;
-        Hacl.Bignum25519.fdifference x3 t0;
-        Hacl.Bignum25519.reduce x3
-      ) else ();
-      blit x3 0ul x 0ul 5ul;
+        make_zero t0;
+        fdifference_norm x3 t0
+      ) else (
+        let h = ST.get() in
+        lemma_modifies_1 h tmp);
+      copy x3 x;
       true
     )
-    else false
+    else (
+      let h = ST.get() in
+      lemma_modifies_2 h x tmp;
+      false)
+  ) in
+  pop_frame();
+  res
+
+
+val recover_x:
+  x:elemB ->
+  y:elemB{disjoint x y} ->
+  sign:UInt64.t{v sign = 0 \/ v sign = 1} ->
+  Stack bool
+    (requires (fun h -> live h x /\ live h y /\ red_51 (as_seq h y)))
+    (ensures (fun h0 z h1 -> live h1 x /\ live h0 y /\ modifies_1 x h0 h1 /\
+      (let op_String_Access = Seq.index in
+       let y = as_seq h0 y in
+       let y:nat = v y.[0] + pow2 51 * v y.[1] + pow2 102 * v y.[2] + pow2 153 * v y.[3]
+               + pow2 204 * v y.[4]in
+       let x = as_seq h1 x in
+       let sign = (v sign = 1) in
+       let res  = Spec.Ed25519.recover_x y sign in True)
+       (* (z <==> Some? res) *)
+       (* /\ (Some? res ==> (seval x = Some?.v res /\ red_51 x))) *)
+      ))
+#reset-options "--max_fuel 0 --z3rlimit 500"
+let recover_x x y sign =
+  assert_norm(pow2 32 = 0x100000000);
+  push_frame();
+  let tmp = create 0uL 20ul in
+  let x2  = Buffer.sub tmp 0ul 5ul in
+  let x3  = Buffer.sub tmp 5ul 5ul in
+  let t0  = Buffer.sub tmp 10ul 5ul in
+  let t1  = Buffer.sub tmp 15ul 5ul in
+  let b = gte_q y in
+  let res =
+  if b then (
+    let hf = ST.get() in
+    lemma_modifies_2 hf x tmp;
+    false
+  ) else (
+    let h = ST.get() in
+    lemma_reveal_seval (as_seq h y);
+    recover_x_step_1 x2 y;
+    Hacl.Impl.Ed25519.Pow2_252m2.pow2_252m2 x3 x2;
+    let h' = ST.get() in
+    lemma_red_513_is_red_5413 (as_seq h' x3);
+    Hacl.Bignum25519.fsquare t0 x3;
+    copy x2 t1;
+    fdifference_norm t1 t0;
+    let t1_is_0 = is_0 t1 in
+    if t1_is_0 then ()
+    else (
+      mul_modp_sqrt_m1 x3
+    );
+    Hacl.Bignum25519.fsquare t0 x3;
+    copy x2 t1;
+    fdifference_norm t1 t0;
+    Hacl.Bignum25519.reduce x3;
+    let t1_is_0 = is_0 t1 in
+    if t1_is_0 then (
+      let x0 = x_mod_2 x3 in
+      (* let x0 = x3.(0ul) &^ 1uL in *)
+      if not(x0 =^ sign) then (
+        make_zero t0;
+        fdifference_norm x3 t0
+      ) else (
+        let h = ST.get() in
+        lemma_modifies_1 h tmp);
+      copy x3 x;
+      true
+    )
+    else (
+      let h = ST.get() in
+      lemma_modifies_2 h x tmp;
+      false)
   ) in
   pop_frame();
   res
