code/experimental/ed25519/Hacl.Impl.Ed25519.PointDecompress.fst
@@ -6,6 +6,7 @@ open Hacl.Bignum25519
 open Hacl.Impl.Ed25519.ExtPoint
 
 
+#reset-options "--max_fuel 0 --z3rlimit 20"
 
 private
 val split_2_255:
