code/experimental/ed25519/Hacl.Impl.Ed25519.Pow2_252m2.fsti
@@ -13,6 +13,6 @@ val pow2_252m2:
   (requires (fun h -> live h out /\ live h z /\ red_513 (as_seq h z)))
   (ensures (fun h0 _ h1 -> live h1 out /\ modifies_1 out h0 h1 /\ live h0 z
     /\ red_513 (as_seq h0 z)
-    /\ Hacl.Spec.Bignum.Bigint.seval (as_seq h1 out) == Spec.Curve25519.(Hacl.Spec.Bignum.Bigint.seval (as_seq h0 z) ** ((prime + 3) / 8))
+    /\ seval (as_seq h1 out) == Spec.Curve25519.(seval (as_seq h0 z) ** ((prime + 3) / 8))
     /\ red_513 (as_seq h1 out)
   ))
