code/experimental/ed25519/Hacl.Impl.SHA512.ModQ.fsti
@@ -1,0 +1,21 @@
+module Hacl.Impl.SHA512.ModQ
+
+open FStar.Buffer
+open Hacl.Impl.BignumQ.Mul
+open Hacl.UInt64
+
+
+#reset-options "--max_fuel 0 --z3rlimit 20"
+
+val sha512_modq:
+  out:qelemB ->
+  input:buffer Hacl.UInt8.t ->
+  len  :UInt32.t{UInt32.v len = length input} ->
+  Stack unit
+        (requires (fun h0 -> live h0 input /\ live h0 out))
+        (ensures  (fun h0 _ h1 -> live h0 input /\ live h1 out /\ modifies_1 out h0 h1 /\
+          Hacl.Spec.BignumQ.Eval.eval_q (as_seq h1 out) == Spec.Ed25519.sha512_modq (as_seq h0 input) /\
+          (let out = as_seq h1 out in let op_String_Access = Seq.index in
+           v (out.[0]) < 0x100000000000000 /\ v (out.[1]) < 0x100000000000000 /\
+           v (out.[2]) < 0x100000000000000 /\ v (out.[3]) < 0x100000000000000 /\
+           v (out.[4]) < 0x100000000000000) ))
